Clean up

src/crypto/aes/GCTR_i.fst
@@ -24,30 +24,9 @@ let rec gctr_encrypt_length (icb:quad32) (plain:list quad32 { 256 * length plain
   =
   gctr_encrypt_recursive_length icb plain alg key 0
 
-(*
-let rec nth_in_bounds_is_some (l:list 'a) (i:int) : Lemma
-  (requires 0 <= i /\ i < length l)
-  (ensures Some? (nth l i))
-  [SMTPat (nth l i)]
-=
-  if i = 0 then ()
-  else nth_in_bounds_is_some (Cons?.tl l) (i - 1)
-
-let nth_in_bounds (l:list 'a) (i:int {0 <= i /\ i < length l}) =
-  nth_in_bounds_is_some l i;
-  Some?.v (nth l i)
-
-let nth_in_bounds_extension (l:list 'a) (i:int {0 < i /\ i < length l}) : Lemma
-  (requires length l > 0)
-  (ensures (nth_in_bounds l i) == (nth_in_bounds (Cons?.tl l) (i - 1)))
-  =
-  ()
-
-#reset-options "--z3rlimit 50"
-*)
-
-let rec gctr_indexed (icb:quad32) (plain:gctr_plain) 
-		     (alg:algorithm) (key:aes_key alg) (i:int) : Lemma
+#reset-options "--use_two_phase_tc true" // Needed so that indexing cipher and plain knows that their lengths are equal
+let rec gctr_indexed_helper (icb:quad32) (plain:gctr_plain) 
+			    (alg:algorithm) (key:aes_key alg) (i:int) : Lemma
   (requires True)
   (ensures (let cipher = gctr_encrypt_recursive icb plain alg key i in
 	    length cipher == length plain /\
@@ -58,111 +37,26 @@ let rec gctr_indexed (icb:quad32) (plain:gctr_plain)
   | [] -> ()
   | hd :: tl ->
       let cipher = gctr_encrypt_recursive icb plain alg key i in  
-      assert (length cipher == length plain);
       let r_cipher = gctr_encrypt_recursive icb tl alg key (i+1) in     
-      assert( Cons?.tl cipher == r_cipher);
-      gctr_indexed icb tl alg key (i+1);
-      let helper (j:int) :   // TODO: Why do I have to add "j < length cipher" below!?
-	Lemma ((0 <= j /\ j < length plain /\ j < length cipher) ==> (index cipher j == quad32_xor (index plain j) (aes_encrypt alg key (inc32 icb (i + j)) )))
+      let helper (j:int) : 
+	Lemma ((0 <= j /\ j < length plain) ==> (index cipher j == quad32_xor (index plain j) (aes_encrypt alg key (inc32 icb (i + j)) )))
 	= 
-	if j <= 0 then ()
-	else if j < length plain then (
-	  //index_extension cipher j;
-	  //assert(index cipher j == index r_cipher (j - 1));
-	  gctr_indexed icb tl alg key (i+1);
+	if 0 < j && j < length plain then (
+	  gctr_indexed_helper icb tl alg key (i+1);
 	  assert(index r_cipher (j-1) == quad32_xor (index tl (j-1)) (aes_encrypt alg key (inc32 icb (i + 1 + j - 1)) )) // OBSERVE
-	  //assert(index plain j == index tl (j-1))
-	) else ()	
+	) else ()
       in
       FStar.Classical.forall_intro helper
 
-#reset-options "--use_two_phase_tc true" // Needed so that indexing cipher and plain knows that their lengths are equal
-let rec gctr_indexed_full (icb:quad32) (plain:gctr_plain) 
+let rec gctr_indexed (icb:quad32) (plain:gctr_plain) 
 		     (alg:algorithm) (key:aes_key alg) (cipher:list quad32) : Lemma
   (requires  length cipher == length plain /\
              (forall i . {:pattern index cipher i} 0 <= i /\ i < length cipher ==> 
 	     index cipher i == quad32_xor (index plain i) (aes_encrypt alg key (inc32 icb i) )))
   (ensures  cipher == gctr_encrypt icb plain alg key)
 =
-  gctr_indexed icb plain alg key 0;
+  gctr_indexed_helper icb plain alg key 0;
   let c = gctr_encrypt_recursive icb plain alg key 0 in
   index_extensionality c cipher;
   ()
 
-
-(*
-
-(*      
-      assert (index r_cipher (i-1) == quad32_xor (index tl (i-1)) (aes_encrypt alg key (inc32 icb (i+1) )));
-      assert( Cons?.tl cipher == r_cipher);
-      //assert (index r_cipher (i-1) == index cipher i);
-      
-      assume(False)
-*)      
-
-
-let rec gctr_indexed (icb:quad32) (plain:gctr_plain) 
-		     (alg:algorithm) (key:aes_key alg) (i:int { 0 <= i /\ i < length plain }) : Lemma
-  (requires True)
-  (ensures (let cipher = gctr_encrypt icb plain alg key in
-	    length cipher == length plain /\
-	   (index cipher i == quad32_xor (index plain i) (aes_encrypt alg key (inc32 icb i) ))))
-=
-  if i = 0 then ()
-  else 
-    match plain with 
-    | [] -> ()
-    | hd :: tl -> 
-      let cipher = gctr_encrypt_recursive icb plain alg key 0 in  
-      let tl_cipher = gctr_encrypt_recursive icb tl alg key 1 in  
-      assert( Cons?.tl cipher == tl_cipher);
-      gctr_indexed icb plain alg key (i - 1);
-      assert (index cipher (i-1) == quad32_xor (index plain (i-1)) (aes_encrypt alg key (inc32 icb (i-1) )));
-      assume(False)
-
-
-      let r_cipher = gctr_encrypt_recursive icb tl alg key (i-1) in     
-      gctr_indexed icb tl alg key (i - 1);
-      assert (index r_cipher (i-1) == quad32_xor (index tl (i-1)) (aes_encrypt alg key (inc32 icb (i+1) )));
-      assert( Cons?.tl cipher == r_cipher);
-      //assert (index r_cipher (i-1) == index cipher i);
-      
-      assume(False)
-
-
-
-
-let rec gctr_indexed (icb:quad32) (plain:gctr_plain) 
-		     (alg:algorithm) (key:aes_key alg) (i:int { 0 <= i /\ i < length plain }) : Lemma
-  (requires True)
-  (ensures (let cipher = gctr_encrypt_recursive icb plain alg key i in
-	    length cipher == length plain /\
-	   (index cipher i == quad32_xor (index plain i) (aes_encrypt alg key (inc32 icb i) ))))
-=
-  if i = 0 then ()
-  else 
-    match plain with 
-    | [] -> ()
-    | hd :: tl -> 
-      let cipher = gctr_encrypt_recursive icb plain alg key i in  
-      let r_cipher = gctr_encrypt_recursive icb tl alg key (i+1) in     
-      gctr_indexed icb tl alg key (i + 1);
-      assert (index r_cipher (i-1) == quad32_xor (index tl (i-1)) (aes_encrypt alg key (inc32 icb (i+1) )));
-      assert( Cons?.tl cipher == r_cipher);
-      //assert (index r_cipher (i-1) == index cipher i);
-      
-      assume(False)
-*)   
-  
-(*
-let rec gctr_equivalence (icb:quad32) (plain:gctr_plain) 
-		     (alg:algorithm) (key:aes_key alg) (cipher:list quad32) : Lemma
-  (requires length cipher == length plain /\
-             (forall i . {:pattern nth cipher i} 0 <= i /\ i < length cipher ==> 
-	     index cipher i == quad32_xor (index plain i) (aes_encrypt alg key (inc32 icb i) )))
-  (ensures  cipher == gctr_encrypt icb plain alg key)
-=
-  match plain with
-  | [] -> ()
-  | hd :: tl -> gctr_equivalence icb tl alg key (Cons?.tl cipher)
-*)
